

$f'(x)=\lim_{h \to 0} \dfrac{f(x+h)-f(x)}{h}$

$\dfrac{d}{dx}[]$

# Rules
Let $f, g$ be functions. Let $c, n$ be constants.



* $\dfrac{d}{dx}[f(x)]=f'(x)$

Constants can be simply moved outside of the differentiation.
$\dfrac{d}{dx}[cf]=c\dfrac{d}{dx}[f]$

Differentiation is linear:
$\dfrac{d}{dx}[f \pm g]=\dfrac{d}{dx}[f] \pm \dfrac{d}{dx}[g]$


$\dfrac{d}{dx}[fg]=f\dfrac{d}{dx}[g]+\dfrac{d}{dx}[f]g$




## Power rule

* $\dfrac{d}{dx}[x^n] = nx^{n-1}$
The more general version is this below:
* $\dfrac{d}{dx}[x^{an+b}] = (an+b)x^{an+b-1}$

In fact, the reason why $\dfrac{d}{dx}[c]=0$ is because $\dfrac{d}{dx}[cx^0]=0cx^{-1}=0$.
## Chain rule
* $\dfrac{d}{dx}[f(g(x))] = f'(g(x))g'(x)$

* $\dfrac{d}{dx}[c^{ax+b}]=ac^{ax+b}\ln(c)$
* $\dfrac{d}{dx}[e^{ax+b}]=ae^{ax+b}\ln(e)=ae^{ax+b}$
* $\dfrac{d}{dx}[\ln(ax+b)]=(ax+b)^{-1}a$
* 


## Misc 0
* $\dfrac{d}{dx}[f(x)]=f'(x)$


